finish base spirea wp rules
with some admits..

src/base/generational_resources.v
@@ -22,17 +22,51 @@ From self.algebra Require Import view.
 
 From self.lang Require Import lang.
 
-Definition crashed_atR : cmra := prodR (agreeR viewO) (agreeR viewO).
-(* Definition crashed_at_inG Σ Ω := genInDepsG Σ Ω crashed_atR []. *)
-Notation crashed_at_inG Σ Ω := (genInDepsG Σ Ω crashed_atR [#]).
-
 (* Names used:
  * - OV: The offset view, the sum of all crash views from prior generations
  * - OCV: The crash view including offsets
  * - OPV: The persist view including offsets
  * - CV: The crash view, CV = OCV - OV
  * - PV: The persist view, PV = OPV - OV
+ * - SV: The store view (also called "lub" view), SV = OSV - OV
  *)
+
+Definition store_viewR : cmra := (authR viewO).
+Notation store_view_inG Σ Ω := (genInDepsG Σ Ω store_viewR [#]).
+
+
+Definition crashed_atR : cmra := prodR (agreeR viewO) (agreeR viewO).
+(* Definition crashed_at_inG Σ Ω := genInDepsG Σ Ω crashed_atR []. *)
+Notation crashed_at_inG Σ Ω := (genInDepsG Σ Ω crashed_atR [#]).
+
+(* All the functors that we need for the base logic (and not ghost names). This
+is identical to [nvmBaseFixedG] except for the [invG] part. *)
+Class nvmBaseG Σ Ω  := NvmBaseG {
+  (* valid view *)
+  nvmBaseG_store_view_in :> store_view_inG Σ Ω;
+  store_view_name : gname;
+  (* crashed at *)
+  nvmBaseG_crashed_at_in :> crashed_at_inG Σ Ω;
+  crashed_at_name : gname;
+  (* persisted *)
+  nvmBaseG_persisted_in :>
+    genInDepsG Σ Ω (authR viewUR) [#crashed_atR];
+    (* persisted_genInG (i := nvmBaseG_crashed_at_in) Σ Ω; *)
+  persisted_name : gname;
+  (* heap map *)
+  nvmBaseG_gmap_view_in :>
+    genInDepsG Σ Ω (gmap_viewR loc (leibnizO (gmap nat message))) [#crashed_atR];
+  (* gmap_view_genInG (i := nvmBaseG_crashed_at_in) Σ Ω; *)
+  heap_name : gname;
+}.
+
+(* has been upstreamed to [iris-nextgen]. *)
+Lemma fmap_auth_auth {A : ucmra} (a : A) t :
+  fmap_auth t (● a) ≡ ● (t a) ⋅ ◯ (t ε).
+Proof.
+  rewrite /fmap_auth /fmap_view view.view_op_eq /=.
+  rewrite right_id left_id /fmap_pair agree_map_to_agree //.
+Qed.
 
 Definition drop_word s := substring (1 + findex 0 " " s) (String.length s) s.
 
@@ -41,9 +75,89 @@ Tactic Notation "iPickedInAgree" constr(Hs) :=
   iDestruct (gen_picked_in_agree with Hs) as %<-;
   iClear na.
 
+Section store_view.
+  (* Resource for lub view *)
+  Context `{!nvmBaseG Σ Ω}.
+  #[local] Notation storeI := (nvmBaseG_store_view_in).
+  #[local] Existing Instance nvmBaseG_store_view_in.
+  (* we don't care about the transformation of valid views since [validV] predicates
+   * are not supposed to survive into next generation anyway. *)
+  Definition store_view_trans : store_viewR → store_viewR :=
+    fmap_auth (const ∅).
+
+  Instance store_view_trans_cmra_morphism :
+    CmraMorphism store_view_trans.
+  Proof.
+    rewrite /store_view_trans.
+    apply @fmap_auth_gentrans, cmra_morphism_const.
+    - apply _.
+    - done.
+    - done.
+  Qed.
+
+  Definition store_view_pred: pred_over store_viewR :=
+    λ t, t = store_view_trans.
+
+  Definition store_view_auth γ SV: iProp Σ :=
+    "store_view_at" ∷ gen_own (i := genInDepsG_gen storeI) γ (● SV) ∗
+    "store_view_tok" ∷ token γ [#] (store_view_pred) (store_view_pred).
+
+  (* Expresses that the view [V] is valid. This means that it is included in the
+   * lub view. *)
+  Definition validV (V : view) : iProp Σ :=
+    gen_own (i := genInDepsG_gen storeI) store_view_name (◯ V).
+
+  Lemma store_view_alloc SV :
+    ⊢ |==> ∃ γ, store_view_auth γ SV.
+  Proof.
+    iMod (own_gen_alloc (DS := [#])
+      (● SV) [#] [##] with "[]") as (γ) "(HO & tok)".
+    { apply auth_auth_valid, view_valid. }
+    { iIntros (i'). inversion i'. }
+    iMod (
+      token_strengthen_promise (DS := [#])
+        _ [#] [##] _ (store_view_pred) _ (store_view_pred) with "[] tok")
+      as "tok".
+    { intros ???. unfold True_rel. rewrite huncurry_curry. done. }
+    { done. }
+    { intros ts. dependent elimination ts. done. }
+    { intros ts _. dependent elimination ts.
+      eexists.
+      split; last done.
+      apply _. }
+    { iIntros (i'). inversion i'. }
+    iModIntro.
+    iExists (γ).
+    iFrame.
+  Qed.
+
+  (** Owning [lub_at] and [store_view_tok] allows us to pick any view in
+   * next generation (after a bupd). *)
+  Lemma store_view_nextgen γ SV1 SV2 :
+    store_view_auth γ SV1 ⊢ ⚡==> |==> store_view_auth γ SV2.
+  Proof.
+    iNamed 1.
+    iDestruct (token_to_rely with "[$]") as "#rely".
+    iModIntro.
+    iDestruct "store_view_at" as "(%t & #picked1 & lub_at)".
+    iDestruct "rely" as "[rely (% & % & (? & ->) & picked2 & ?)]".
+    iDestruct (gen_picked_in_agree with "picked1 picked2") as %->.
+
+    rewrite /store_view_trans fmap_auth_auth /=.
+    iDestruct (gen_own_op with "lub_at") as "[lub_at _]".
+    iFrame.
+    iMod (own_update with "lub_at") as "$"; last done.
+    apply gen_cmra_update; try done.
+    apply option_update, auth_auth_grow; first apply view_valid.
+    apply view_empty_least.
+  Qed.
+End store_view.
+
 Section crashed_at.
   (* Resource for crashed at view *)
-  Context `{caI : !crashed_at_inG Σ Ω}.
+  Context `{!nvmBaseG Σ Ω}.
+  #[local] Existing Instance nvmBaseG_crashed_at_in.
+  #[local] Notation caI := nvmBaseG_crashed_at_in.
 
   (* The transition function that gets applied to the crashed at view at a
    * crash. [OCV2] is the news offset crash view. *)
@@ -74,15 +188,26 @@ Section crashed_at.
   Definition crashed_at_pred (OPV : view) : pred_over crashed_atR :=
     λ t, ∃ OCV2, OPV ⊑ OCV2 ∧ t = crashed_at_trans OCV2.
 
+  Definition crashed_at_pred_strengthen OCV1 OCV2:
+    OCV2 ⊑ OCV1 →
+    pred_stronger (crashed_at_pred OCV1) (crashed_at_pred OCV2).
+  Proof.
+    intros.
+    intros t (OPV & ? & ?).
+    exists OPV.
+    split; last done.
+    by trans OCV1.
+  Qed.
+
   Definition crashed_at_rel PV : rel_over [#] crashed_atR :=
     crashed_at_pred PV.
 
-  Definition crashed_at_both γ OV OCV : iProp Σ :=
-    gen_own (i := genInDepsG_gen caI) γ (to_agree OV, to_agree OCV).
+  Definition crashed_at_both OV OCV : iProp Σ :=
+    gen_own (i := genInDepsG_gen caI) crashed_at_name (to_agree OV, to_agree OCV).
 
-  Lemma crashed_at_both_agree γ OV1 OCV1 OV2 OCV2 :
-    crashed_at_both γ OV1 OCV1 -∗
-    crashed_at_both γ OV2 OCV2 -∗
+  Lemma crashed_at_both_agree OV1 OCV1 OV2 OCV2 :
+    crashed_at_both OV1 OCV1 -∗
+    crashed_at_both OV2 OCV2 -∗
     ⌜ OV1 = OV2 ⌝ ∗ ⌜ OCV1 = OCV2 ⌝.
   Proof.
     iIntros "O1 O2".
@@ -97,23 +222,46 @@ Section crashed_at.
   Qed.
 
   (* Ownership over the offest crashed at view. *)
-  Definition crashed_at_offset γ OCV : iProp Σ :=
-    ∃ OV, gen_own γ (to_agree OV, to_agree OCV).
+  Definition crashed_at_offset OCV : iProp Σ :=
+    ∃ OV, gen_own crashed_at_name (to_agree OV, to_agree OCV).
 
-  Definition crashed_at γ (CV : view) : iProp Σ :=
+  Lemma crashed_at_offset_agree OCV OCV' :
+    crashed_at_offset OCV -∗ crashed_at_offset OCV' -∗ ⌜OCV = OCV'⌝.
+  Proof.
+    iIntros "[% H1] [% H2]".
+    iDestruct (gen_own_valid_2 with "H1 H2") as "%eq".
+    rewrite pair_valid ?to_agree_op_valid_L in eq.
+    destruct eq as [-> ->].
+    done.
+  Qed.
+
+  Definition crashed_at (CV : view) : iProp Σ :=
     ∃ (OV OCV LV : view),
       (* "%view_add" ∷ ⌜ OV `view_add` CV = OCV ⌝ ∗ *)
       "%view_eq" ∷ ⌜ OCV `view_sub` OV = CV ⌝ ∗
-      "agree" ∷ gen_own γ (to_agree OV, to_agree OCV)
+      "agree" ∷ gen_own crashed_at_name (to_agree OV, to_agree OCV)
       (* ∗ "rely" ∷ rely γ [] (crashed_at_pred LV) (crashed_at_pred LV). *)
-      ∗ "rely" ∷ rely_self γ (crashed_at_pred LV).
+      ∗ "rely" ∷ rely_self crashed_at_name (crashed_at_pred LV).
 
+  Lemma crashed_at_agree CV CV' :
+    crashed_at CV -∗ crashed_at CV' -∗ ⌜CV = CV'⌝.
+  Proof.
+    iNamed 1.
+    iIntros "(% & % & % & % & agree' & _)".
+    simplify_eq.
+    iPoseProof (gen_own_op with "[$agree $agree']") as "agree".
+    iDestruct (gen_own_valid with "[$]") as "%eq".
+    rewrite pair_valid ?to_agree_op_valid_L in eq.
+    destruct eq as [-> ->].
+    done.
+  Qed.
+  
   (** Ownership over the crashed at token with a promise that after the next
    * crash the [OCV] will be at least [LV]. *)
   Definition crashed_at_tok γ LV : iProp Σ :=
     token γ [#] (crashed_at_pred LV) (crashed_at_pred LV).
 
-  Lemma crashed_at_tok_strengthen γ LV1 LV2 :
+  Lemma crashed_at_tok_strengthen {γ} LV1 LV2 :
     LV1 ⊑ LV2 →
     crashed_at_tok γ LV1 ⊢ |==> crashed_at_tok γ LV2.
   Proof.
@@ -126,39 +274,53 @@ Section crashed_at.
       eexists LV2. done.
   Qed.
 
-  Lemma crashed_at_alloc CV :
-    ⊢ |==> ∃ γ, crashed_at γ CV ∗ crashed_at_tok γ CV.
+  Definition crashed_at_auth_crashed_at OV OCV LV:
+    crashed_at_tok crashed_at_name LV -∗
+    crashed_at_both OV OCV -∗
+    crashed_at (OCV `view_sub` OV).
   Proof.
-    iMod (own_gen_alloc (DS := [#])
-      (to_agree ∅, to_agree CV) [#] [##] with "[]") as (γ) "(HO & tok)".
-    { done. }
-    { iIntros (i'). inversion i'. }
-    iMod (
-      token_strengthen_promise (DS := [#])
-        _ [#] [##] _ (crashed_at_pred CV) _ (crashed_at_pred CV) with "[] tok")
-      as "tok".
-    { intros ???. unfold True_rel. rewrite huncurry_curry. done. }
-    { done. }
-    { intros ts. dependent elimination ts. done. }
-    { intros ts _. dependent elimination ts.
-      exists (λ '(_, CV1), (CV1, to_agree CV)).
-      split; first apply _.
-      exists CV. done. }
-    { iIntros (i'). inversion i'. }
-    iModIntro.
-    iExists (γ).
-    iDestruct (token_to_rely with "tok") as "#R".
-    iFrame.
-    iExists ∅, CV, _. iFrame.
-    iDestruct (rely_to_rely_self with "R") as "$".
-    iPureIntro.
-    apply view_sub_empty.
+    iIntros.
+    rewrite /crashed_at_both /crashed_at_tok.
+    iPoseProof (token_to_rely with "[$]") as "?".
+    iPoseProof (rely_to_rely_self with "[$]") as "?".
+    iExists _, _, _.
+    iFrame "∗#".
+    done.
   Qed.
+
+  (* Lemma crashed_at_alloc CV : *)
+  (*   ⊢ |==> ∃ γ, crashed_at γ CV ∗ crashed_at_tok γ CV. *)
+  (* Proof. *)
+  (*   iMod (own_gen_alloc (DS := [#]) *)
+  (*     (to_agree ∅, to_agree CV) [#] [##] with "[]") as (γ) "(HO & tok)". *)
+  (*   { done. } *)
+  (*   { iIntros (i'). inversion i'. } *)
+  (*   iMod ( *)
+  (*     token_strengthen_promise (DS := [#]) *)
+  (*       _ [#] [##] _ (crashed_at_pred CV) _ (crashed_at_pred CV) with "[] tok") *)
+  (*     as "tok". *)
+  (*   { intros ???. unfold True_rel. rewrite huncurry_curry. done. } *)
+  (*   { done. } *)
+  (*   { intros ts. dependent elimination ts. done. } *)
+  (*   { intros ts _. dependent elimination ts. *)
+  (*     exists (λ '(_, CV1), (CV1, to_agree CV)). *)
+  (*     split; first apply _. *)
+  (*     exists CV. done. } *)
+  (*   { iIntros (i'). inversion i'. } *)
+  (*   iModIntro. *)
+  (*   iExists (γ). *)
+  (*   iDestruct (token_to_rely with "tok") as "#R". *)
+  (*   iFrame. *)
+  (*   iExists ∅, CV, _. iFrame. *)
+  (*   iDestruct (rely_to_rely_self with "R") as "$". *)
+  (*   iPureIntro. *)
+  (*   apply view_sub_empty. *)
+  (* Qed. *)
 
   (** Owning [crashed_at] gives [crashed_at] for some view in the next
    * generation. *)
-  Lemma crashed_at_nextgen γ CV :
-    crashed_at γ CV ⊢ ⚡==> ∃ CV2, crashed_at γ CV2.
+  Lemma crashed_at_nextgen CV :
+    crashed_at CV ⊢ ⚡==> ∃ CV2, crashed_at CV2.
   Proof.
     iNamed 1.
     iModIntro.
@@ -175,13 +337,13 @@ Section crashed_at.
     iPureIntro. reflexivity.
   Qed.
 
-  Lemma crashed_at_pick_nextgen γ OV OCV OCV2 LV :
+  Lemma crashed_at_pick_nextgen OV OCV OCV2 LV :
     LV ⊑ OCV2 →
-    crashed_at_both γ OV OCV -∗
-    crashed_at_tok γ LV -∗
+    crashed_at_both OV OCV -∗
+    crashed_at_tok crashed_at_name LV -∗
     |==> ⚡==>
-      crashed_at_both γ OCV OCV2 ∗ crashed_at_tok γ LV ∗
-      picked_in γ (crashed_at_trans OCV2).
+      crashed_at_both OCV OCV2 ∗ crashed_at_tok crashed_at_name LV ∗
+      picked_in crashed_at_name (crashed_at_trans OCV2).
   Proof.
     iIntros (le) "AG tok".
     unfold crashed_at_tok, crashed_at_offset.
@@ -197,11 +359,7 @@ Section crashed_at.
     iPickedInAgree "picked picked2".
     simpl. naive_solver.
   Qed.
-
 End crashed_at.
-
-Definition persisted_genInG Σ Ω `{i : !crashed_at_inG Σ Ω} :=
-  genInDepsG Σ Ω (authR viewUR) [#crashed_atR].
 
 #[global]
 Instance genInSelfG_one Σ Ω A :
@@ -235,10 +393,10 @@ Section rules_one_dep.
 End rules_one_dep.
 
 Section persisted.
-  Context `{!crashed_at_inG Σ Ω}.
-  Context `{i : !persisted_genInG Σ Ω}.
-  Context (persist_view_name : gname).
-  Context (crashedγ : gname).
+  Context `{!nvmBaseG Σ Ω}.
+  #[local] Existing Instance nvmBaseG_crashed_at_in.
+  #[local] Notation i := nvmBaseG_persisted_in.
+  #[local] Existing Instance nvmBaseG_persisted_in.
 
   Local Definition persisted_rel : rel_over [#crashed_atR] (authR viewUR) :=
     λ tC tP,
@@ -247,17 +405,9 @@ Section persisted.
         tP = fmap_auth (const OCV).
 
   Definition persisted_auth OPV : iProp Σ :=
-    gen_own (i := genInDepsG_gen i) persist_view_name (● OPV) ∗
-    rely (g := i) persist_view_name [#crashedγ] persisted_rel (λ _, true).
+    gen_own (i := genInDepsG_gen i) persisted_name (● OPV) ∗
+    rely (g := i) persisted_name [#crashed_at_name] persisted_rel (λ _, true).
     (* ∗ rely_self crashedγ (crashed_at_pred OPV). *)
-
-  (* has been upstreamed to [iris-nextgen]. *)
-  Lemma fmap_auth_auth {A : ucmra} (a : A) t :
-    fmap_auth t (● a) ≡ ● (t a) ⋅ ◯ (t ε).
-  Proof.
-    rewrite /fmap_auth /fmap_view view.view_op_eq /=.
-    rewrite right_id left_id /fmap_pair agree_map_to_agree //.
-  Qed.
 
   #[global]
   Instance persisted_auth_into_nextgen OPV :
@@ -265,7 +415,7 @@ Section persisted.
       (persisted_auth OPV)
       (∃ OCV2,
         persisted_auth OCV2 ∗
-        picked_in crashedγ (crashed_at_trans OCV2)).
+        picked_in crashed_at_name (crashed_at_trans OCV2)).
       (* (∃ OCV2, ⌜ OPV ⊑ OCV2 ⌝ ∗ persisted_auth (OPV `view_add` CV)). *)
   Proof.
     rewrite /IntoNextgen /persisted_auth.
@@ -282,15 +432,87 @@ Section persisted.
   Qed.
 
   Definition persisted PV : iProp Σ :=
-    ∃ OCV OPV,
+    ∃ OCV OPV OPV',
       "%view_eq" ∷ ⌜ OPV `view_sub` OCV = PV ⌝ ∗
-      "agree" ∷ crashed_at_offset crashedγ OCV ∗
-      "persLub" ∷ gen_own (i := genInDepsG_gen i) persist_view_name (◯ OPV) ∗
-      "crashRely" ∷ rely_self crashedγ (crashed_at_pred OPV) ∗
-      "rely" ∷ rely (g := i) persist_view_name [#crashedγ] persisted_rel (λ _, true).
+      "#agree" ∷ crashed_at_offset OCV ∗
+      "#persLub" ∷ gen_own (i := genInDepsG_gen i) persisted_name (◯ OPV) ∗
+      "%actualOPV" ∷ ⌜ OPV ⊑ OPV' ⌝ ∗
+      "#crashRely" ∷ rely_self crashed_at_name (crashed_at_pred OPV') ∗
+      "#rely" ∷ rely (g := i) persisted_name [#crashed_at_name] persisted_rel (λ _, true).
 
-  (* Lemma persisted_weak PV PV' : PV' ≼ PV → persisted PV -∗ persisted PV'. *)
-  (* Proof. ... Qed. *)
+  Lemma persisted_auth_included OCV OPV PV' :
+    crashed_at_offset OCV -∗
+    persisted_auth OPV -∗
+    persisted PV' -∗
+    ⌜PV' ⊑ OPV `view_sub` OCV ⌝.
+  Proof.
+    iIntros "[% crashed_at] [auth _] persisted".
+    iNamed "persisted".
+    iDestruct (gen_own_valid_2 with "auth persLub") as %[_ [incl _]]%auth_both_dfrac_valid_discrete.
+    iDestruct "agree" as "[% crashed_at']".
+    iDestruct (gen_own_valid_2 with "crashed_at crashed_at'") as %[_ <-%to_agree_op_valid_L]%pair_valid.
+    iPureIntro.
+    simplify_eq.
+    by apply view_sub_mono.
+  Qed.
+
+  Lemma persisted_weak PV1 PV2 : PV2 ≼ PV1 → persisted PV1 -∗ persisted PV2.
+  Proof.
+    intros H.
+    iNamed 1.
+    set OPV2 := (map_imap (λ ℓ t, Some (MaxNat (match PV1 !! ℓ with
+                                                | Some (MaxNat 0) => 0
+                                                | _ => (max_nat_car t + (OCV !!0 ℓ))
+                                                end))) PV2).
+    iExists OCV, OPV2, OPV'.
+    iFrame "#".
+    iSplit; first iPureIntro.
+    { rewrite /view_sub map_imap_compose /=.
+      apply map_eq.
+      intros j.
+      rewrite map_lookup_imap /=.
+      rewrite -subseteq_view_incl view_included in H.
+      specialize (H j).
+      destruct (PV2 !! j) as [[n2] | ]; last done.
+      simpl.
+      do 2 f_equiv.
+      destruct (PV1 !! j) as [[[ | n1]] | ].
+      - apply Some_MaxNat_included in H.
+        lia.
+      - lia.
+      - apply option_not_included_None in H.
+        done. }
+    assert (le: OPV2 ⊑ OPV). {
+      apply view_included.
+      intros j.
+      rewrite -subseteq_view_incl view_included in H.
+      specialize (H j).
+      simplify_eq. subst OPV2.
+      rewrite /view_sub map_lookup_imap /= in H.
+      rewrite /view_sub !map_lookup_imap /=.
+      destruct (PV2 !! j) as [ [n1] | ]; destruct (OPV !! j) as [ [n2] | ]; simpl in *; try done.
+      - apply Some_MaxNat_included in H.
+        apply Some_MaxNat_included.
+        destruct (n2 - (OCV !!0 j)) eqn:?; lia.
+      - apply option_not_included_None in H.
+        done.
+      - apply option_included_total.
+        by left. }
+    iSplit.
+    { rewrite /named.
+      rewrite -(gen_own_mono _ _ (◯ OPV2)); first iApply "persLub".
+      apply auth_frag_mono, le. }
+    iPureIntro.
+    etrans; first apply le.
+    done.
+  Qed.
+
+  Global Instance persisted_persistent PV : Persistent (persisted PV).
+  Proof. apply _. Qed.
+
+  (* [persisted] is anti-monotone. *)
+  Global Instance persisted_anti_mono : Proper ((⊑@{view}) ==> flip (⊢)) (persisted).
+  Proof. intros ???. iApply persisted_weak. done. Qed.
 
   Lemma view_sub_something OPV OCV2 OCV :
     OPV ⊑ OCV2 →
@@ -307,7 +529,7 @@ Section persisted.
   Instance persisted_into_nextgen PV :
     IntoNextgen
       (persisted PV)
-      (persisted (view_to_zero PV) ∗ ∃ CV, ⌜PV ⊑ CV⌝ ∗ crashed_at crashedγ CV).
+      (persisted (view_to_zero PV) ∗ ∃ CV, ⌜PV ⊑ CV⌝ ∗ crashed_at CV).
   Proof.
     rewrite /IntoNextgen.
     iNamed 1.
@@ -329,25 +551,22 @@ Section persisted.
     rewrite bi.sep_exist_l.
     iExists (OCV2 `view_sub` OCV).
     assert (PV ⊑ OCV2 `view_sub` OCV).
-    { rewrite -view_eq. apply view_sub_mono. done. }
+    { rewrite -view_eq. apply view_sub_mono. by trans OPV'. }
     iSplit.
-    { iExists OCV2, OPV. iFrame. simpl.
+    { iExists OCV2, OPV, OPV'. iFrame "#%". simpl.
       rewrite fmap_auth_frag. simpl.
       iSplit.
       { iPureIntro. rewrite -view_eq.
-        apply view_sub_something. done. }
-      iSplit. { iExists _. iFrame. }
+        apply view_sub_something. by trans OPV'. }
+      iSplit. { iExists _. iFrame "#". }
       iApply (gen_own_mono with "persLub").
-      Search auth_frag "view".
-      destruct incl as (V & ->).
-      exists (◯ V). done. }
-    iFrame.
+      apply auth_frag_mono.
+      by trans OPV'. }
     iSplit; first done.
     iExists _, _, _.
-    iFrame.
+    iFrame "#".
     done.
   Qed.
-
 End persisted.
 
 Definition gmap_view_genInG Σ Ω `{i : !genInDepsG Σ Ω crashed_atR [#] } :=
@@ -355,16 +574,16 @@ Definition gmap_view_genInG Σ Ω `{i : !genInDepsG Σ Ω crashed_atR [#] } :=
 
 (* Resources and transformation for the heap. *)
 
-Definition heapR : cmra := gmap_viewR loc (leibnizO history).
-
 Section heap.
   (* The transformation of the heap depends on the transformation of the
    * crashed_at view. *)
-  Context `{!genInDepsG Σ Ω crashed_atR [#] }.
-  (* Context {V : Type}. *)
-  Context `{i : !genInDepsG Σ Ω heapR [#crashed_atR] }.
-  Context (crashedγ : gname).
+  Context `{!nvmBaseG Σ Ω}.
+  #[local] Existing Instance nvmBaseG_gmap_view_in.
+  #[local] Existing Instance nvmBaseG_crashed_at_in.
+  #[local] Notation i := nvmBaseG_crashed_at_in.
+  #[local] Definition heapR : cmra := gmap_viewR loc (leibnizO history).
 
+  (* Context {V : Type}. *)
   (* Given a new [OCV] we can define the transformation applied to the history
    * [hist] at each key [l]. *)
   Definition drop_above_hist (OCV : view) (l : loc)
@@ -386,53 +605,264 @@ Section heap.
       tC = crashed_at_trans OCV ∧
       tP = map_entry_lift_gmap_view (drop_above_hist OCV).
 
-  Definition own_auth_heap heapγ heap : iProp Σ :=
+  Definition own_auth_heap heap : iProp Σ :=
     ∃ OCV,
-      "own_auth" ∷ gen_own heapγ (gmap_view_auth (DfracOwn 1) heap) ∗
-      "crashed" ∷ crashed_at_offset crashedγ OCV ∗
+      "own_auth" ∷ gen_own heap_name (gmap_view_auth (DfracOwn 1) heap) ∗
+      "#crashed" ∷ crashed_at_offset OCV ∗
       (* We only keep the rely as we never want to strengthen the promise and
        * never want to pick anything (the promise itself completely determines
        * the transformation). *)
-      "rely" ∷ rely heapγ [#crashedγ] heap_rel (λ _, true).
+      "#rely" ∷ rely heap_name [#crashed_at_name] heap_rel (λ _, true).
        (* "tok" ∷ token heapγ [crashedγ] heap_rel True_pred. *)
 
-  Lemma own_auth_heap_alloc LV heap OCV :
-    crashed_at_offset crashedγ OCV -∗
-    rely_self crashedγ (crashed_at_pred LV) ==∗
-    ∃ heapγ, own_auth_heap heapγ heap.
+  (* [f(ull-)mapsto] is the mapsto predicate containing the entire history
+   * in the ghost resource, while [mapsto] only assert over the current generation
+   * history *)
+  Definition fmapsto (ℓ: loc) (dq: dfrac) (h_full: leibnizO history): iProp Σ :=
+    gen_own heap_name (gmap_view_frag ℓ dq h_full).
+
+  Definition mapsto (ℓ: loc) (dq: dfrac) (h: leibnizO history): iProp Σ :=
+    ∃ OCV (h_full: leibnizO history), "crashed_at_offset" ∷ crashed_at_offset OCV ∗
+                  "%drop_prefix_eq" ∷ ⌜ h = drop_prefix h_full (OCV !!0 ℓ) ⌝ ∗
+                  "fmapsto" ∷ fmapsto ℓ dq h_full.
+
+  (* [hist] might have locations that are not in [OCV]. Hence we cannot use
+   * [map_zip_with] here. *)
+  (* Definition store_drop_prefix OCV (hist : store) := *)
+  (*   map_imap (λ l h, Some $ drop_prefix h (OCV !!0 l)) hist. *)
+  (* The [map_imap] definition is giving me a lot of trouble with
+   * [heap_array] related lemmas. I'm restating it with [map_zip_with]
+   * and manual padding *)
+
+  Definition store_drop_prefix OCV (hist : store) :=
+    map_zip_with
+      (λ h '(MaxNat n), drop_prefix h n)
+      hist
+      (OCV ⊔ (view_to_zero $ max_view hist)).
+
+  Lemma store_drop_prefix_alt ℓ OCV hist:
+    (store_drop_prefix OCV hist) !! ℓ = (λ h, drop_prefix h (OCV !!0 ℓ)) <$> hist !! ℓ.
   Proof.
-    iIntros "crashed #rely".
-    iMod (own_gen_alloc (DS := [#_])
-      (gmap_view_auth (DfracOwn 1) heap)
-      [#crashedγ] [##crashed_at_pred LV] with "[]") as (γ) "[HH tok]".
-    { apply gmap_view_auth_valid. }
-    { iIntros (i').
-      dependent elimination i' as [0%fin].
-      iApply "rely". }
-    iMod (
-      token_strengthen_promise (DS := [#_])
-        _ [#_] [##_] _ heap_rel _ True_pred with "[] tok")
-      as "tok".
-    { intros ???. unfold True_rel. rewrite huncurry_curry. done. }
-    { done. }
-    { intros ts. dependent elimination ts. done. }
-    2: {
-      iIntros (i').
-      dependent elimination i' as [0%fin].
-      iApply "rely". }
-    { intros ts crashedPred.
-      dependent elimination ts as [hcons tC hnil].
-      destruct crashedPred as ((OCV2 & ? & ->) & _).
-      exists (map_entry_lift_gmap_view (drop_above_hist OCV2)).
-      split; first apply _.
-      simpl.
-      exists OCV2. done. }
-    iModIntro.
-    iExists γ, OCV.
-    unfold own_auth_heap.
-    iFrame.
-    iDestruct (token_to_rely with "tok") as "$".
+    rewrite map_lookup_zip_with lookup_op ?lookup_fmap /lookup_zero /=.
+    destruct (hist !! ℓ) as [? | ] eqn:Heqn; last done.
+    simpl.
+    set v := (OCV !! ℓ).
+    destruct v; last done.
+    simpl.
+    rewrite Nat.max_0_r //.
   Qed.
+
+  Lemma dom_store_drop_prefix OCV hist:
+    dom $ store_drop_prefix OCV hist = dom hist.
+  Proof.
+    rewrite dom_map_zip_with_L /view_to_zero dom_op ?dom_fmap_L /=.
+    set_solver.
+  Qed.
+
+  Lemma disjoint_store_drop_prefix V store:
+    dom V ## dom store →
+    store_drop_prefix V store = store.
+  Proof.
+    intros.
+    rewrite /store_drop_prefix.
+    apply map_eq.
+    intros ℓ.
+    rewrite map_lookup_zip_with lookup_op ?lookup_fmap /=.
+    set v := (V !! ℓ).
+    destruct (store !! ℓ) as [ h | ] eqn:Heqn; last done.
+    simpl.
+    apply elem_of_dom_2 in Heqn.
+    assert (v = None) as ->
+                         by (apply not_elem_of_dom; set_solver).
+    rewrite /= drop_prefix_zero //.
+  Qed.
+
+  Lemma store_drop_prefix_union OCV store1 store2:
+    store1 ##ₘ store2 →
+    store_drop_prefix OCV (store1 ∪ store2) =
+    store_drop_prefix OCV store1 ∪ store_drop_prefix OCV store2.
+  Proof.
+    intros H.
+    rewrite /store_drop_prefix.
+    apply map_eq.
+    intros ℓ.
+    rewrite ?map_lookup_zip_with ?lookup_op ?lookup_fmap /=.
+    destruct ((store1 ∪ store2) !! ℓ) eqn:Heqn; simpl.
+    - rewrite map_disjoint_alt in H.
+      destruct (H ℓ) as [ ? | ? ].
+      + rewrite lookup_union_r;
+          rewrite ?map_lookup_zip_with ?lookup_op ?lookup_fmap /=;
+          simplify_map_eq; last done.
+        rewrite lookup_union_r in Heqn; last done.
+        simplify_map_eq.
+        set v := (OCV !! ℓ).
+        by destruct v.
+      + rewrite lookup_union_l;
+          rewrite ?map_lookup_zip_with ?lookup_op ?lookup_fmap /=;
+          simplify_map_eq; last done.
+        rewrite lookup_union_l in Heqn; last done.
+        simplify_map_eq.
+        set v := (OCV !! ℓ).
+        by destruct v.
+    - symmetry.
+      apply lookup_union_None.
+      apply lookup_union_None in Heqn as [??].
+      rewrite ?map_lookup_zip_with ?lookup_op ?lookup_fmap /=.
+      simplify_map_eq.
+      done.
+  Qed.
+
+  Lemma insert_store_drop_prefix ℓ t v hist hist' OCV store:
+    ℓ ∈ dom store →
+    hist' = (drop_prefix hist (OCV !!0 ℓ)) →
+    store_drop_prefix OCV (<[ℓ := <[ t + (OCV !!0 ℓ) := v ]> hist]>store) =
+    <[ℓ := <[ t := v ]> hist' ]> (store_drop_prefix OCV store).
+  Proof.
+    intros.
+    subst hist'.
+    set t' := t + (OCV !!0 ℓ).
+    replace t with (t' - (OCV !!0 ℓ)) by lia.
+    rewrite drop_prefix_insert.
+    rewrite Nat.sub_add; last lia.
+    rewrite /store_drop_prefix.
+    set padded_view := (e in map_zip_with _ (insert _ _ _) e).
+    replace padded_view with (<[ℓ := MaxNat (OCV !!0 ℓ)]> padded_view).
+    - rewrite -map_insert_zip_with.
+      do 3 f_equal.
+      apply view_to_zero_dom_eq.
+      rewrite ?dom_fmap_L dom_insert_L.
+      set_solver.
+    - apply insert_id.
+      rewrite lookup_op /=.
+      rewrite (view_to_zero_dom_eq _ (max_view store)).
+      2: { rewrite ?dom_fmap_L dom_insert_L.
+           set_solver. }
+      erewrite view_to_zero_lookup.
+      2: { apply (lookup_lookup_total_dom (Inhabited0 := populate (MaxNat 0))).
+           rewrite ?dom_fmap_L //. }
+      rewrite /lookup_zero.
+      set v' := (OCV !! ℓ).
+      destruct v' as [[?] | ]; simpl; last done.
+      rewrite -Some_op max_nat_op Nat.max_0_r //.
+  Qed.
+
+  (* [gen_heap] lemmas, probably better put into typeclass instances later *)
+
+  Lemma fmapsto_heap_valid heap ℓ dq h_full:
+    own_auth_heap heap -∗ fmapsto ℓ dq h_full -∗ ⌜ heap !! ℓ = Some h_full ⌝.
+  Proof.
+    iIntros "heap fmapsto".
+    iNamed "heap".
+    iDestruct (gen_own_valid_2 with "own_auth fmapsto") as %[_ [_ look]]%gmap_view_both_dfrac_valid_L.
+    done.
+  Qed.
+
+  Lemma mapsto_heap_valid OCV heap ℓ dq h:
+    crashed_at_offset OCV -∗ own_auth_heap heap -∗ mapsto ℓ dq h -∗ ⌜ store_drop_prefix OCV heap !! ℓ = Some h ⌝.
+  Proof.
+    iIntros "crashed_at_offset' heap mapsto".
+    iNamed "mapsto".
+    iDestruct (crashed_at_offset_agree with "crashed_at_offset crashed_at_offset'") as "->".
+    iDestruct (fmapsto_heap_valid with "[$] [$]") as %look.
+    iPureIntro.
+    rewrite store_drop_prefix_alt look /=.
+    by f_equiv.
+  Qed.
+
+  Lemma heap_alloc_fmapsto σ ℓ h_full :
+    σ !! ℓ = None →
+    own_auth_heap σ ==∗ own_auth_heap (<[ℓ:=h_full]>σ) ∗ fmapsto ℓ (DfracOwn 1) h_full.
+  Proof.
+    iIntros (Hσl).
+    iNamed 1.
+    iMod (gen_own_update with "own_auth") as "[own_auth frag]".
+    { eapply (gmap_view.gmap_view_alloc _ _ (DfracOwn 1)); [ apply Hσl | done ]. }
+    iFrame.
+    iModIntro.
+    iExists _.
+    iFrame "#".
+  Qed.
+
+  Lemma heap_alloc_big_fmapsto σ σ' :
+    σ' ##ₘ σ →
+    own_auth_heap σ ==∗
+    own_auth_heap (σ' ∪ σ) ∗ ([∗ map] ℓ ↦ h_full ∈ σ', fmapsto ℓ(DfracOwn 1) h_full).
+  Proof.
+    revert σ; induction σ' as [| ℓ v σ' Hl IH] using map_ind; iIntros (σ Hdisj) "Hσ".
+    { rewrite left_id_L. auto. }
+    iMod (IH with "Hσ") as "[Hσ'σ Hσ']"; first by eapply map_disjoint_insert_l.
+    decompose_map_disjoint.
+    rewrite !big_opM_insert // -insert_union_l //.
+    by iMod (heap_alloc_fmapsto with "Hσ'σ") as "[$ $]";
+    first by apply lookup_union_None.
+  Qed.
+
+  Lemma fmapsto_heap_update σ ℓ h_full1 h_full2:
+    own_auth_heap σ -∗
+    fmapsto ℓ (DfracOwn 1) h_full1 ==∗
+    own_auth_heap (<[ℓ:=h_full2]>σ) ∗ fmapsto ℓ (DfracOwn 1) h_full2.
+  Proof.
+    iNamed 1.
+    iIntros "fmapsto".
+    iMod (gen_own_update_2 with "own_auth fmapsto") as "[$ $]".
+    { apply gmap_view_update. }
+    iModIntro.
+    iExists _.
+    iFrame "#".
+  Qed.
+
+  Lemma mapsto_heap_update OCV σ ℓ h1 h_full2:
+    crashed_at_offset OCV -∗
+    own_auth_heap σ -∗
+    mapsto ℓ (DfracOwn 1) h1 ==∗
+    own_auth_heap (<[ℓ := h_full2]>σ) ∗
+    mapsto ℓ (DfracOwn 1) (drop_prefix h_full2 (OCV !!0 ℓ)).
+  Proof.
+    iIntros "#crashed_at_offset' auth". iNamed 1.
+    iDestruct (crashed_at_offset_agree with "crashed_at_offset crashed_at_offset'") as "->".
+    iMod (fmapsto_heap_update with "[$] [$]") as "[$ fmapsto]".
+    iExists _, _.
+    iFrame.
+    done.
+  Qed.
+
+  (* Lemma own_auth_heap_alloc LV heap OCV : *)
+  (*   crashed_at_offset OCV -∗ *)
+  (*   rely_self crashed_at_name (crashed_at_pred LV) ==∗ *)
+  (*   ∃ heapγ, own_auth_heap heapγ heap. *)
+  (* Proof. *)
+  (*   iIntros "crashed #rely". *)
+  (*   iMod (own_gen_alloc (DS := [#_]) *)
+  (*     (gmap_view_auth (DfracOwn 1) heap) *)
+  (*     [#crashed_at_name] [##crashed_at_pred LV] with "[]") as (γ) "[HH tok]". *)
+  (*   { apply gmap_view_auth_valid. } *)
+  (*   { iIntros (i'). *)
+  (*     dependent elimination i' as [0%fin]. *)
+  (*     iApply "rely". } *)
+  (*   iMod ( *)
+  (*     token_strengthen_promise (DS := [#_]) *)
+  (*       _ [#_] [##_] _ heap_rel _ True_pred with "[] tok") *)
+  (*     as "tok". *)
+  (*   { intros ???. unfold True_rel. rewrite huncurry_curry. done. } *)
+  (*   { done. } *)
+  (*   { intros ts. dependent elimination ts. done. } *)
+  (*   2: { *)
+  (*     iIntros (i'). *)
+  (*     dependent elimination i' as [0%fin]. *)
+  (*     iApply "rely". } *)
+  (*   { intros ts crashedPred. *)
+  (*     dependent elimination ts as [hcons tC hnil]. *)
+  (*     destruct crashedPred as ((OCV2 & ? & ->) & _). *)
+  (*     exists (map_entry_lift_gmap_view (drop_above_hist OCV2)). *)
+  (*     split; first apply _. *)
+  (*     simpl. *)
+  (*     exists OCV2. done. } *)
+  (*   iModIntro. *)
+  (*   iExists γ, OCV. *)
+  (*   unfold own_auth_heap. *)
+  (*   iFrame. *)
+  (*   iDestruct (token_to_rely with "tok") as "$". *)
+  (* Qed. *)
 
   Lemma map_entry_lift_gmap_view_auth dq
       (heap : gmap loc (leibnizO history)) map_entry :
@@ -443,11 +873,11 @@ Section heap.
     rewrite agree_map_to_agree. done.
   Qed.
 
-  Lemma own_auth_heap_nextgen heapγ heap :
-    own_auth_heap heapγ heap
+  Lemma own_auth_heap_nextgen heap :
+    own_auth_heap heap
     ⊢ ⚡==> ∃ OCV,
-      crashed_at_offset crashedγ OCV ∗
-      own_auth_heap heapγ (drop_above_map OCV heap).
+      crashed_at_offset OCV ∗
+      own_auth_heap (drop_above_map OCV heap).
   Proof.
     iNamed 1.
     iModIntro.
@@ -458,60 +888,58 @@ Section heap.
     iPickedInAgree "pickedH pickedH'".
     destruct rel as (OCV2 & -> & ->).
     iExists OCV2.
+    iFrame "#".
     iSplit.
-    { iExists _. iFrame. }
-    { iExists _. iFrame.
-      iSplit. 2: { iExists _. iFrame. }
+    { iExists _. iFrame "#". }
+    { iExists _.
+      iSplit. 2: { iExists _. iFrame "#". }
       rewrite map_entry_lift_gmap_view_auth.
       iFrame. }
   Qed.
 
   #[global]
-  Instance into_nextgen_own_auth_heap heapγ heap : IntoNextgen _ _ :=
-    own_auth_heap_nextgen heapγ heap.
-
+  Instance into_nextgen_own_auth_heap heap : IntoNextgen _ _ :=
+    own_auth_heap_nextgen heap.
 End heap.
 
-(* All the functors that we need for the base logic (and not ghost names). This
-is identical to [nvmBaseFixedG] except for the [invG] part. *)
-Class nvmBaseG Σ Ω  := NvmBaseG {
-  (* crashed at *)
-  nvmBaseG_crashed_at_in :> crashed_at_inG Σ Ω;
-  crashed_at_name : gname;
-  (* persisted *)
-  nvmBaseG_persisted_in :>
-    genInDepsG Σ Ω (authR viewUR) [#crashed_atR];
-    (* persisted_genInG (i := nvmBaseG_crashed_at_in) Σ Ω; *)
-  persisted_name : gname;
-  (* heap map *)
-  nvmBaseG_gmap_view_in :>
-    genInDepsG Σ Ω (gmap_viewR loc (leibnizO (gmap nat message))) [#crashed_atR];
-  (* gmap_view_genInG (i := nvmBaseG_crashed_at_in) Σ Ω; *)
-  heap_name : gname;
-}.
+Notation "l ↦fh{ dq } v" := (fmapsto l dq (v%V))
+  (at level 20, format "l  ↦fh{ dq }  v") : bi_scope.
+Notation "l ↦fh□ v" := (fmapsto l DfracDiscarded (v%V))
+  (at level 20, format "l  ↦fh□  v") : bi_scope.
+Notation "l ↦fh{# q } v" := (fmapsto l (DfracOwn q) (v%V))
+  (at level 20, format "l  ↦fh{# q }  v") : bi_scope.
+Notation "l ↦fh v" := (fmapsto l (DfracOwn 1) (v%V))
+  (at level 20, format "l  ↦fh  v") : bi_scope.
 
-Search drop_prefix.
-(* [hist] might have locations that are not in [OCV]. Hence we cannot use
- * [map_zip_with] here. *)
-Definition store_drop_prefix OCV (hist : store) :=
-  map_imap (λ l h, Some $ drop_prefix h (OCV !!0 l)) hist.
+Notation "l ↦h{ dq } v" := (mapsto l dq (v%V))
+  (at level 20, format "l  ↦h{ dq }  v") : bi_scope.
+Notation "l ↦h□ v" := (mapsto l DfracDiscarded (v%V))
+  (at level 20, format "l  ↦h□  v") : bi_scope.
+Notation "l ↦h{# q } v" := (mapsto l (DfracOwn q) (v%V))
+  (at level 20, format "l  ↦h{# q }  v") : bi_scope.
+Notation "l ↦h v" := (mapsto l (DfracOwn 1) (v%V))
+  (at level 20, format "l  ↦h  v") : bi_scope.
 
 (* The state interpretation for the base logic. *)
 Definition nvm_heap_ctx `{!nvmBaseG Σ Ω} (σ : mem_config) : iProp Σ :=
   ∃ (OV OCV : view) (full_hist : store),
+    (* store view *)
+    "store_view_auth" ∷ store_view_auth store_view_name (max_view σ.1) ∗
     (* crashed at *)
     "%full_hist_eq" ∷ ⌜ σ.1 = store_drop_prefix OCV full_hist ⌝ ∗
     "%Hop" ∷ ⌜ valid_heap σ.1 ⌝ ∗
-    "crashed" ∷ gen_own crashed_at_name (to_agree OV, to_agree OCV) ∗
+    "#crashed" ∷ gen_own crashed_at_name (to_agree OV, to_agree OCV) ∗
     (* The lower bound on the next [OCV] is the current [OCV] plus [PV]. *)
     "crashed_at_tok" ∷ crashed_at_tok crashed_at_name (OCV `view_add` σ.2) ∗
     (* The interpretation of the heap. *)
-    "Hσ" ∷ own_auth_heap crashed_at_name heap_name full_hist ∗
+    "Hσ" ∷ own_auth_heap full_hist ∗
     (* [OCV] is "the sum of all crash views". The domain of the crash views
      * only grows and is always included in the persist view. And hence the
-     * domain of the persist view also contains the domain of [OCV]. *)
-    "%ocvDom" ∷ ⌜ dom OCV ⊆ dom σ.2 ⌝ ∗
-    "pers" ∷ persisted_auth (i := nvmBaseG_persisted_in) persisted_name crashed_at_name (OCV `view_add` σ.2).
+     * domain of the persist view also contains the domain of [OCV].
+     * Furthermore, the domain of persist view is always smaller than the
+     * heap itself. *)
+    "%ocvDom" ∷ ⌜ dom OCV ⊆ dom σ.2 ∧ dom OCV ⊆ dom σ.1 ⌝ ∗
+    "pers" ∷ persisted_auth (OCV `view_add` σ.2).
 
 Lemma view_add_lookup_zero V1 V2 ℓ :
   (V1 `view_add` V2) !!0 ℓ = (V1 !!0 ℓ) + (V2 !!0 ℓ).
@@ -528,16 +956,16 @@ Lemma slice_of_store_drop_prefix CV OCV full_hist :
 Proof.
   intros sub.
   apply map_eq => ℓ.
-  rewrite /store_drop_prefix.
   rewrite /slice_of_store.
   rewrite /slice_of_hist.
   rewrite 2!lookup_fmap.
   rewrite /drop_above_map.
-  rewrite 2!map_lookup_imap.
+  rewrite !store_drop_prefix_alt.
+  rewrite !map_lookup_imap.
   rewrite /slice_hist.
   rewrite map_zip_with_flip.
-  rewrite map_lookup_zip_with.
-  rewrite map_lookup_imap.
+  rewrite {1}map_lookup_zip_with.
+  rewrite store_drop_prefix_alt.
   destruct (full_hist !! ℓ) eqn:look; rewrite look; simpl; last done.
   unfold drop_above_hist.
   rewrite !view_add_lookup_zero.
@@ -591,27 +1019,30 @@ Proof.
   intros [store PV CV pIncl cut].
   unfold nvm_heap_ctx. simpl.
   iNamed 1.
-  iMod (crashed_at_pick_nextgen _ _ _ (OCV `view_add` CV)
-    with "crashed crashed_at_tok") as "crashed".
+  iMod (crashed_at_pick_nextgen _ _ (OCV `view_add` CV)
+    with "crashed crashed_at_tok") as "crashed'".
   { f_equiv. done. }
-  iModIntro. iModIntro.
-  iDestruct "crashed" as "(#crashed & crashed_at_tok & pickedC)".
-  iMod (crashed_at_tok_strengthen _ _ (OCV `view_add` CV) with "crashed_at_tok") as "tok".
+  iModIntro.
+  iPoseProof (store_view_nextgen _ _ (max_view (slice_of_store CV store)) with "[$]") as "store_view_auth".
+  iModIntro.
+  iMod "store_view_auth".
+  iDestruct "crashed'" as "(#crashed' & crashed_at_tok & pickedC)".
+  iMod (crashed_at_tok_strengthen _ (OCV `view_add` CV) with "crashed_at_tok") as "tok".
   { f_equiv. done. }
   iModIntro.
   set (OCV2 := OCV `view_add` CV).
-  iDestruct ("Hσ") as (?) "[(% & crashed') Hσ]".
-  iDestruct (crashed_at_both_agree with "crashed' crashed") as "[-> ->]".
+  iDestruct ("Hσ") as (?) "[(% & crashed'') Hσ]".
+  iDestruct (crashed_at_both_agree with "crashed'' crashed'") as "[-> ->]".
   iExists OCV, OCV2, _.
-  iFrame "Hσ".
+  iFrame "Hσ store_view_auth".
   apply view_le_dom_subseteq in pIncl.
   iSplit.
   { iPureIntro. rewrite full_hist_eq.
     rewrite /OCV2.
     apply slice_of_store_drop_prefix.
-    etrans; done. }
+    trans (dom CV); set_solver. }
   iSplit. { iPureIntro. apply store_inv_cut; done. }
-  iFrame "crashed". simpl.
+  iFrame "crashed''". simpl.
   rewrite -(assoc view_add).
   rewrite view_add_view_zero.
   iFrame "tok".
@@ -626,6 +1057,9 @@ Proof.
   rewrite view_add_dom.
   rewrite /view_to_zero.
   rewrite dom_fmap.
+  split; first set_solver.
+  subst.
+  apply consistent_cut_subseteq_dom in cut.
+  rewrite /slice_of_store /slice_of_hist !dom_fmap_L dom_map_zip_with_L.
   set_solver.
 Qed.
-
