perennial/base_logic/lib/wsat.v
@@ -3,7 +3,6 @@ From iris.algebra Require Import gmap auth agree gset coPset list vector excl.
 From Perennial.algebra Require Import mlist.
 From iris.proofmode Require Import tactics.
 From self.nextgen Require Import nextgen_promises_ng.
-From self.base Require Import generational_resources.
 From Perennial.base_logic Require Export lib.own lib.later_credits.
 From iris.prelude Require Import options.
 
