src/program_logic/lifting.v
@@ -1,0 +1,111 @@
+(** The "lifting lemmas" in this file serve to lift the rules of the operational
+semantics to the program logic. *)
+
+From iris.proofmode Require Import tactics.
+From self.program_logic Require Export crash_weakestpre.
+From iris.prelude Require Import options.
+
+Section lifting.
+Context `{!irisGS Λ Σ Ω}.
+Implicit Types s : stuckness.
+Implicit Types v : val Λ.
+Implicit Types e : expr Λ.
+Implicit Types σ : state Λ.
+Implicit Types P Q : iProp Σ.
+Implicit Types Φ : val Λ → iProp Σ.
+
+Local Hint Resolve reducible_no_obs_reducible : core.
+
+(* Lemma wp_lift_step_ncfupdN s E Φ e1 : *)
+(*   to_val e1 = None → *)
+(*   (∀ σ1 g1 ns mj D κ κs nt, state_interp σ1 nt -∗ global_state_interp g1 ns mj D (κ ++ κs) -∗ |={E,∅}=> *)
+(*     |={∅}▷=>^(S $ num_laters_per_step ns) *)
+(*     ⌜if s is NotStuck then reducible e1 σ1 g1 else True⌝ ∗ *)
+(*     ∀ e2 σ2 g2 efs, ⌜prim_step e1 σ1 g1 κ e2 σ2 g2 efs⌝ -∗ *)
+(*       £ (S $ num_laters_per_step ns) *)
+(*        -∗ |NC={∅,E}=> *)
+(*       state_interp σ2 (length efs + nt) ∗ *)
+(*       global_state_interp g2 (step_count_next ns) mj D κs ∗ *)
+(*       WP e2 @ s; E {{ Φ }} ∗ *)
+(*       [∗ list] ef ∈ efs, WP ef @ s; ⊤ {{ fork_post }}) *)
+(*   ⊢ WP e1 @ s; E {{ Φ }}. *)
+(* Proof. *)
+(*   rewrite wp_eq /wp_def !wpc_unfold /wpc_pre=>->. *)
+(*   iIntros "H" (mj). iSplit; last first. *)
+(*   { iIntros. iApply step_fupd_extra.step_fupd2N_inner_later; auto. iNext; iFrame. } *)
+(*   iIntros (????????) "Hσ Hg HNC Hlc". *)
+(*   iSpecialize ("H" with "[$] [$]"). *)
+(*   rewrite ncfupd_eq. *)
+(*   iMod ("H" with "[$]") as "(H&HNC)". *)
+(*   iMod (fupd2_mask_subseteq ∅ ∅) as "Hclo"; [set_solver+..|]. *)
+(*   iModIntro. iApply step_fupd_extra.step_fupdN_step_fupd2N. *)
+(*   iApply (step_fupdN_wand with "H"). iIntros "($&H)". *)
+(*   iIntros. iMod "Hclo". iMod ("H" with "[//] Hlc [$]") as "(($ & $ & He & Hef)&HNC)". *)
+(*   iModIntro. iFrame. iSplitL "He". *)
+(*   - iApply wpc0_wpc. *)
+(*     iApply (wpc_strong_mono' with "[$]"); auto. *)
+(*     destruct (to_val); set_solver. *)
+(*   - iApply (big_sepL_mono with "Hef")=>???/=. iApply wpc0_wpc. *)
+(* Qed. *)
+
+Lemma wp_lift_step_fupdN s E Φ e1 :
+  to_val e1 = None →
+  (∀ σ1 g1 ns mj D κ κs nt, state_interp σ1 nt -∗ global_state_interp g1 ns mj D (κ ++ κs) -∗ |={E,∅}=>
+    |={∅}▷=>^(S $ num_laters_per_step ns)
+    ⌜if s is NotStuck then reducible e1 σ1 g1 else True⌝ ∗
+    ∀ e2 σ2 g2 efs, ⌜prim_step e1 σ1 g1 κ e2 σ2 g2 efs⌝ -∗
+      £ (S $ num_laters_per_step ns)
+       -∗ |={∅,E}=>
+      state_interp σ2 (length efs + nt) ∗
+      global_state_interp g2 (step_count_next ns) mj D κs ∗
+      WP e2 @ s; E {{ Φ }} ∗
+      [∗ list] ef ∈ efs, WP ef @ s; ⊤ {{ fork_post }})
+  ⊢ WP e1 @ s; E {{ Φ }}.
+Proof.
+Admitted.
+
+Lemma wp_lift_step_fupd s E Φ e1 :
+  to_val e1 = None →
+  (∀ σ1 g1 ns mj D κ κs nt, state_interp σ1 nt -∗ global_state_interp g1 ns mj D (κ ++ κs) ={E,∅}=∗ ▷
+    (⌜if s is NotStuck then reducible e1 σ1 g1 else True⌝ ∗
+    ∀ e2 σ2 g2 efs, ⌜prim_step e1 σ1 g1 κ e2 σ2 g2 efs⌝ -∗
+      £ (S $ num_laters_per_step ns)
+      ={∅,E}=∗
+      state_interp σ2 (length efs + nt) ∗
+      global_state_interp g2 (step_count_next ns) mj D κs ∗
+      WP e2 @ s; E {{ Φ }} ∗
+      [∗ list] ef ∈ efs, WP ef @ s; ⊤ {{ fork_post }}))
+  ⊢ WP e1 @ s; E {{ Φ }}.
+Proof.
+  intros ?. rewrite -wp_lift_step_fupdN; [|done]. simpl.
+  iIntros "H". iIntros (????????) "Hσ Hg".
+  iMod ("H" with "[$] [$]") as "(Hr&N)".
+  iModIntro.
+  iApply step_fupdN_intro; first done.
+  iModIntro. iNext. iModIntro. iNext. eauto.
+Qed.
+
+Lemma wp_lift_atomic_step {s E Φ} e1 :
+  to_val e1 = None →
+  (∀ σ1 g1 ns mj D κ κs nt, state_interp σ1 nt -∗ global_state_interp g1 ns mj D (κ ++ κs) ={E}=∗
+    ⌜if s is NotStuck then reducible e1 σ1 g1 else True⌝ ∗
+    ▷ ∀ e2 σ2 g2 efs, ⌜prim_step e1 σ1 g1 κ e2 σ2 g2 efs⌝ -∗
+      £ (S (num_laters_per_step ns))
+      ={E}=∗
+      state_interp σ2 (length efs + nt) ∗
+      global_state_interp g2 (step_count_next ns) mj D κs ∗
+      from_option Φ False (to_val e2) ∗
+      [∗ list] ef ∈ efs, WP ef @ s; ⊤ {{ fork_post }})
+  ⊢ WP e1 @ s; E {{ Φ }}.
+Proof.
+  iIntros (?) "H".
+  iApply (wp_lift_step_fupd s E _ e1)=>//; iIntros (σ1 g1 ns mj D κ κs nt) "Hσ1 Hg1".
+  iMod ("H" with "[$] [$]") as "[$ H]".
+  iApply fupd_mask_intro; first set_solver.
+  iIntros "Hclose". iNext.
+  iIntros (e2 ???) "%Hstep Hlater". iMod "Hclose". iMod ("H" with "[//] [$]") as "($ & $ & H & ?)".
+  destruct (to_val e2) eqn:?; last by iExFalso.
+  iFrame. iModIntro. iApply wp_value; last done. by apply of_to_val.
+Qed.
+
+End lifting.
